# Week 10 class
![[Week 10 exercise 1.png]]
a)
$$|A|=1*4-3*2=4-5=-1$$
b)
$$|A|=0-(-3*3)=0-(-6)=6$$
c)
$$|A|=6-0=6$$
d)
$$|A|=0-0+1*(15-18)=-3$$
e)
$$|A|=1*(6*(-2))=-12$$
f)
$$|A|=1*(6*4)=24$$
g)
$$|A|=1*(6*4)=24$$
h)
$$|A|= A_{1,1}-A_{1,2} \cdot 0+A_{1,3}= -6+-6=-12$$
i)
$$|A|=0$$
l)
$$|A|=36-0+(-36)-0=36-36=0$$
![[Week 10 excersice 2.png]]

a) 
$$\vec{x}= [2*3-3*0, 3*1-1*3, 1*0-2*1]=[6, 0, -2]$$
b)
$[5][3][7]$
$[1][0][0]$

$$\vec{x}= [0, 7-0, 0-3]=[0,7,-3]$$
![[Week 10 exercise 3.png]]
a)
$$A^{-1}=\frac{1}{|A|}\begin{pmatrix}4 & -2 \\ -3 & 1\end{pmatrix}
= \frac{1}{4-5}\begin{pmatrix}4 & -2 \\ -3 & 1\end{pmatrix}
= 1/-1\begin{pmatrix}4 & -2 \\ -3 & 1\end{pmatrix}
= -\begin{pmatrix}4 & -2 \\ -3 & 1\end{pmatrix}
= \begin{pmatrix}-4 & 2 \\ 3 & -1\end{pmatrix}$$
b) 
$$A^{-1}=
1/9\begin{pmatrix}0 & -3 \\ 3 & 0\end{pmatrix}
=\begin{pmatrix}0 & -\frac{1}{3} \\ 1/3 & 0\end{pmatrix}$$
c)
$$A^{-1}
=\frac{1}{6}\begin{pmatrix}6 & 0 \\ -3 & 1\end{pmatrix}
=\begin{pmatrix}1 & 0 \\ -\frac{1}{2} &  \frac{1}{6}\end{pmatrix}$$
d)

e)
$$A^{-1}=
\begin{pmatrix}
1 & 0 & 0 \\ 
0 & 6 & 0 \\ 
0 & 0 & -2
\end{pmatrix}$$
I multiply row 2 by 1/6 and row 3 by -1/2


$$\begin{pmatrix}
1 & 0 & 0 \\ 
0 & 1 & 0 \\ 
0 & 0 & 1
\end{pmatrix}$$




$$
\newcommand{\dx}{\:\mathrm{d}x}
\newcommand{\md}{\mathrm{d}}
\newcommand{\dfdx}{\frac{\md}{\dx}}
\begin{align*}
\text{given that:} \\	
    \exp(x) &:= \sum_{n=0}^\infty \frac{x^n}{n!},\\[8pt]  
\text{show that:}\\
    \dfdx \exp(x) &= \exp(x), \\
    \dfdx \sum_{n=0}^\infty \frac{x^n}{n!}=\sum_{n=0}^\infty\frac{nx^{n-1}}{n!}=\sum_{n=0}^\infty \frac{x^{n-1}}{(n-1)!}=\sum_{n=0}^\infty \frac{x^n}{n!}, \\ 
    \dfdx1+x+\frac{x^2}{1*2}+\frac{x^3}{1*2*3}+...=1+\frac{2x^1}{1*2}+\frac{3x^2}{1*2*3}+...=1+\frac{x}{1}+\frac{x^2}{1*2}+...
\end{align*}
$$
$$
\newcommand{\dx}{\:\mathrm{d}x}
\newcommand{\md}{\mathrm{d}}
\newcommand{\dfdx}{\frac{\md}{\dx}}
\begin{align*}
    \exp(x) &:= \sum_{n=0}^\infty \frac{x^n}{n!},\\[8pt]  
    \sin(x) &:= \sum_{n=0}^\infty \frac{(-1)^nx^{2n+1}}{(2n+1)!}, \\[8pt]
    \cos(x) &:= \sum_{n=0}^\infty \frac{(-1)^nx^{2n}}{(2n)!}.
\end{align*}
$$
$$
\newcommand{\dx}{\:\mathrm{d}x}
\newcommand{\md}{\mathrm{d}}
\newcommand{\dfdx}{\frac{\md}{\dx}}
\begin{align*}
    \exp(x) &:= \sum_{n=0}^\infty \frac{x^n}{n!},\\[8pt]  
    \sin(x) &:= \sum_{n=0}^\infty \frac{(-1)^nx^{2n+1}}{(2n+1)!}, \\[8pt]
    \cos(x) &:= \sum_{n=0}^\infty \frac{(-1)^nx^{2n}}{(2n)!}.
\end{align*}
$$



$$\sin(x) := \sum_{n=0}^\infty \frac{(-1)^nx^{2n+1}}{(2n+1)!}$$
